Example3.v
@@ -60,81 +60,100 @@ Module Export ST <: state.T.
   
   Module Export Ty <: STATE R.
 
-    Module Export D := DFAFn TabT. 
-    
-    Definition State := regex.
-    Definition defState := EmptySet.
-    Definition Delta : Type := TabT.TabTy.Table * TabT.R.Defs.reFS.t.
-    (* State + Delta = DFA, but now the lookup table is separate from the state *)
-    
-    Definition transition (a : Sigma) (e : State) (d : Delta) : State :=
-      let (x,y) := d in
-      match DFAtransition a (e,x,y) with
-        (e',x',y') => e'
-      end.
-    Fixpoint transition_list (bs : list Sigma) (fsm : State) (d : Delta) : State :=
-      let (x,y) := d in
-      match DFAtransition_list bs (fsm, x, y) with
-        (e', x', y') => e'
-      end.
-    
-    Definition accepts (z : String) (e : State) (d : Delta) : bool :=
-      let (x,y) := d in DFAaccepts z (e,x,y).
-    Definition accepting (e : State) (d : Delta) : bool :=
-      let (x,y) := d in DFAaccepting (e,x,y).
+      Module Export D := DFAFn TabT. 
+      
+      Definition State := regex.
+      Definition defState := EmptySet.
+      
+      Definition Delta : Type := TabT.TabTy.Table * TabT.R.Defs.reFS.t.
+      (* State + Delta = DFA, but now the lookup table is separate from the state *)
+      Definition defDelta : Delta := (TabT.TabTy.emptyTable, TabT.TabTy.reFS.empty).
+      Definition init_delta (e : regex) : Delta :=
+        match regex2dfa e with
+          (e', x, y) => (x,y)
+        end.
+      
+      Definition transition (a : Sigma) (e : State) (d : Delta) : State :=
+        let (x,y) := d in
+        match DFAtransition a (e,x,y) with
+          (e',x',y') => e'
+        end.
+      Fixpoint transition_list (bs : list Sigma) (fsm : State) (d : Delta) : State :=
+        let (x,y) := d in
+        match DFAtransition_list bs (fsm, x, y) with
+          (e', x', y') => e'
+        end.
 
-    Lemma accepts_nil: forall(fsm : State) d, accepting fsm d = accepts [] fsm d.
-    Proof. intros fsm. reflexivity. Qed.
+      Lemma transition_list_nil : forall fsm d,
+          transition_list [] fsm d = fsm.
+      Admitted.
+      Lemma transition_list_cons : forall bs a fsm d,
+          transition_list (a :: bs) fsm d = transition_list bs (transition a fsm d) d.
+      Admitted.
+      
+      Definition accepts (z : String) (e : State) (d : Delta) : bool :=
+        let (x,y) := d in DFAaccepts z (e,x,y).
+      Definition accepting (e : State) (d : Delta) : bool :=
+        let (x,y) := d in DFAaccepting (e,x,y).
 
-    Lemma accepts_transition : forall cand a fsm d,
-        accepts cand (transition a fsm d) d = accepts (a :: cand) fsm d.
-    Proof.
-      intros. unfold accepts. destruct d. unfold transition. simpl. repeat dm.
-      - inv E. auto.
-      - inv E. auto.
-    Qed.
+      Lemma accepts_nil: forall(fsm : State) d, accepting fsm d = accepts [] fsm d.
+      Proof. intros fsm. reflexivity. Qed.
 
-    Definition init_state (r : regex) : State := r.
-    Definition init_state_inv (r : State) : regex := r.
-    Definition init_delta (e : regex) : Delta :=
-      match regex2dfa e with
-        (e', x, y) => (x,y)
-      end.
-    
-    Lemma invert_init_correct : forall r s,
-        exp_match s (init_state_inv (init_state r)) <-> exp_match s r.
-    Proof. intros. simpl. unfold init_state. unfold init_state_inv. reflexivity. Qed.
-    
-    Lemma accepts_matches : forall(s : String) (e : regex),
-        true = accepts s (init_state e) (init_delta e) <-> exp_match s e.
-    Proof.
-      split; intros.
-      - symmetry in H. apply r2d_accepts_match.
-        unfold accepts in *. unfold init_state in *. unfold init_delta in *.
-        repeat dm. repeat inj_all. apply transition_Table_correct in E0.
-        destruct E0 as (H0 & H1 & H2). rewrite H1 in *. rewrite <- H2 in *.
-        rewrite accepts_matchb in *; auto.
-        pose proof (TabT.Defs.FillTable.canon_equiv e). unfold re_equiv in *.
-        symmetry in H. symmetry. rewrite Mat.match_iff_matchb in *. apply H3; auto.
-      - symmetry. apply r2d_accepts_match in H. 
-        unfold accepts in *. unfold init_state in *. unfold init_delta in *.
-        repeat dm. repeat inj_all. apply transition_Table_correct in E0.
-        destruct E0 as (H0 & H1 & H2). rewrite H1 in *. rewrite <- H2 in *.
-        rewrite accepts_matchb in *; auto.
-        pose proof (TabT.Defs.FillTable.canon_equiv e). unfold re_equiv in *.
-        symmetry in H. symmetry. rewrite Mat.match_iff_matchb in *. apply H3; auto.
-    Qed.
+      Lemma accepts_transition : forall cand a fsm e d,
+          accepts cand (transition a fsm (init_delta e)) d
+          = accepts (a :: cand) fsm d.
+      Proof.
+        intros. unfold accepts. destruct d. unfold transition.
+        unfold init_delta in *.
+        repeat dm. inv E. (* lots of stuff to unify *)
+      Admitted.
 
-    Definition accepting_dt_list : forall bs e d,
-        d = (init_delta e)
-        -> accepting (transition_list bs (init_state e) d) d
-          = accepting (init_state (derivative_list bs e)) d.
-    Proof.
-      intros. unfold init_state. unfold accepting. unfold init_delta in *.
-      rewrite H. repeat dm. try apply DFAaccepting_dt_list.
-    Admitted.
-    
-  End Ty.
+      Definition init_state (r : regex) : State := r.
+      Definition init_state_inv (r : State) : regex := r.
+      
+      Lemma invert_init_correct : forall r s,
+          exp_match s (init_state_inv (init_state r)) <-> exp_match s r.
+      Proof. intros. simpl. unfold init_state. unfold init_state_inv. reflexivity. Qed.
+      
+      Lemma accepts_matches :  forall(s : String) (e e': regex),
+          true = accepts s (init_state e) (init_delta e') <-> exp_match s e.
+      Admitted.
+      (*Proof.
+        split; intros.
+        - symmetry in H. apply r2d_accepts_match.
+          unfold accepts in *. unfold init_state in *. unfold init_delta in *.
+          repeat dm. repeat inj_all. apply transition_Table_correct in E0.
+          destruct E0 as (H0 & H1 & H2). rewrite H1 in *. rewrite <- H2 in *.
+          rewrite accepts_matchb in *; auto.
+          pose proof (TabT.Defs.FillTable.canon_equiv e). unfold re_equiv in *.
+          symmetry in H. symmetry. rewrite Mat.match_iff_matchb in *. apply H3; auto.
+        - symmetry. apply r2d_accepts_match in H. 
+          unfold accepts in *. unfold init_state in *. unfold init_delta in *.
+          repeat dm. repeat inj_all. apply transition_Table_correct in E0.
+          destruct E0 as (H0 & H1 & H2). rewrite H1 in *. rewrite <- H2 in *.
+          rewrite accepts_matchb in *; auto.
+          pose proof (TabT.Defs.FillTable.canon_equiv e). unfold re_equiv in *.
+          symmetry in H. symmetry. rewrite Mat.match_iff_matchb in *. apply H3; auto.
+      Qed.*)
+
+      Definition accepting_dt_list : forall bs e0 e1 e2,
+      accepting (transition_list bs (init_state e0) (init_delta e1)) (init_delta e2)
+        = accepting (init_state (derivative_list bs e0)) (init_delta e2).
+      Admitted.
+
+      
+      Definition stt_compare (s1 s2 : State) : comparison :=
+        re_compare s1 s2.
+
+      Lemma stt_compare_eq : forall x y,
+          stt_compare x y = Eq <-> x = y.
+      Proof. apply re_compare_eq. Qed.
+
+      Lemma stt_compare_trans : forall c x y z,
+          stt_compare x y = c -> stt_compare y z = c -> stt_compare x z = c.
+      Proof. apply re_compare_trans. Qed.
+      
+    End Ty.
     
   Module Export Defs := state.DefsFn R Ty.
 
